theories/Base.v
@@ -41,6 +41,7 @@ From Katamaran Require Export
      Tactics.
 From Katamaran Require Import
      Syntax.Expressions
+     Syntax.Messages
      Syntax.Patterns
      Syntax.Terms
      Symbolic.Instantiation
@@ -54,7 +55,7 @@ Module Type BaseMixin (Import TY : Types).
     ExpressionsOn TY <+
     TermsOn TY <+ PatternsOn TY <+
     OccursCheckOn TY <+ InstantiationOn TY <+
-    PartialEvaluationOn TY.
+    MessagesOn TY <+ PartialEvaluationOn TY.
 
   Notation PCtx := (NCtx PVar Ty).
   Notation LCtx := (NCtx LVar Ty).
