theories/Syntax/Messages.v
@@ -1,0 +1,106 @@
+(******************************************************************************)
+(* Copyright (c) 2022 Steven Keuchel                                          *)
+(* All rights reserved.                                                       *)
+(*                                                                            *)
+(* Redistribution and use in source and binary forms, with or without         *)
+(* modification, are permitted provided that the following conditions are     *)
+(* met:                                                                       *)
+(*                                                                            *)
+(* 1. Redistributions of source code must retain the above copyright notice,  *)
+(*    this list of conditions and the following disclaimer.                   *)
+(*                                                                            *)
+(* 2. Redistributions in binary form must reproduce the above copyright       *)
+(*    notice, this list of conditions and the following disclaimer in the     *)
+(*    documentation and/or other materials provided with the distribution.    *)
+(*                                                                            *)
+(* THIS SOFTWARE IS PROVIDED BY THE COPYRIGHT HOLDERS AND CONTRIBUTORS        *)
+(* "AS IS" AND ANY EXPRESS OR IMPLIED WARRANTIES, INCLUDING, BUT NOT LIMITED  *)
+(* TO, THE IMPLIED WARRANTIES OF MERCHANTABILITY AND FITNESS FOR A PARTICULAR *)
+(* PURPOSE ARE DISCLAIMED. IN NO EVENT SHALL THE COPYRIGHT HOLDER OR          *)
+(* CONTRIBUTORS BE LIABLE FOR ANY DIRECT, INDIRECT, INCIDENTAL, SPECIAL,      *)
+(* EXEMPLARY, OR CONSEQUENTIAL DAMAGES (INCLUDING, BUT NOT LIMITED TO,        *)
+(* PROCUREMENT OF SUBSTITUTE GOODS OR SERVICES; LOSS OF USE, DATA, OR         *)
+(* PROFITS; OR BUSINESS INTERRUPTION) HOWEVER CAUSED AND ON ANY THEORY OF     *)
+(* LIABILITY, WHETHER IN CONTRACT, STRICT LIABILITY, OR TORT (INCLUDING       *)
+(* NEGLIGENCE OR OTHERWISE) ARISING IN ANY WAY OUT OF THE USE OF THIS         *)
+(* SOFTWARE, EVEN IF ADVISED OF THE POSSIBILITY OF SUCH DAMAGE.               *)
+(******************************************************************************)
+
+From Coq Require Import
+     Bool.Bool
+     Classes.Morphisms
+     Classes.RelationClasses
+     Program.Basics
+     Program.Tactics
+     ZArith.
+
+From Katamaran Require Import
+     Context
+     Environment
+     Notations
+     Prelude
+     Symbolic.OccursCheck
+     Syntax.BinOps
+     Syntax.Terms
+     Syntax.TypeDecl
+     Syntax.Variables
+     Tactics.
+
+From Equations Require Import
+     Equations.
+
+Import ctx.notations.
+Import env.notations.
+
+Local Set Implicit Arguments.
+
+Module Type MessagesOn
+  (Import TY : Types)
+  (Import TM : TermsOn TY)
+  (Import OC : OccursCheckOn TY TM).
+
+  Local Notation LCtx := (NCtx LVar Ty).
+
+  Module amsg.
+    Inductive AMessage (Σ : LCtx) : Type :=
+    | mk {M} {subM : Subst M} {subLM : SubstLaws M} {occM: OccursCheck M} (msg : M Σ)
+    | there {b} (msg : AMessage (Σ ▻ b)).
+    #[global] Arguments mk {_ _ _ _ _} msg.
+    #[global] Arguments there {_ _} msg.
+
+    Fixpoint close {Σ ΣΔ} {struct ΣΔ} : AMessage (Σ ▻▻ ΣΔ) -> AMessage Σ :=
+      match ΣΔ with
+      | []      => fun msg => msg
+      | ΣΔ  ▻ b => fun msg => close (there msg)
+      end%ctx.
+
+    #[export] Instance subst_amessage : Subst AMessage :=
+      fix sub {Σ} m {Σ2} ζ {struct m} :=
+        match m with
+        | mk msg    => mk (subst msg ζ)
+        | there msg => there (sub msg (sub_up1 ζ))
+        end.
+
+    #[export] Instance substlaws_amessage : SubstLaws AMessage.
+    Proof.
+      constructor.
+      - intros ? m. induction m; cbn; f_equal;
+          rewrite ?sub_up1_id; auto using subst_sub_id.
+      - intros ? ? ? ? ? m. revert Σ1 ζ1 Σ2 ζ2.
+        induction m; cbn; intros; f_equal;
+          rewrite ?sub_up1_comp; auto using subst_sub_comp.
+    Qed.
+
+    Import option.notations.
+    #[export] Instance occurscheck_amessage : OccursCheck AMessage :=
+      fix oc {Σ x} xIn m {struct m} :=
+        match m with
+        | mk msg    => mk <$> occurs_check xIn msg
+        | there msg => there <$> oc (ctx.in_succ xIn) msg
+        end.
+
+  End amsg.
+  Export amsg (AMessage).
+  Export (hints) amsg.
+
+End MessagesOn.
